---
title: "Bayesian Reliability Analysis"
author: "Bryant Chen"
date: 2022-01-02
categories: ["Blog"]
tags: ["Simulation", "Bayesian", "Reliability","Mathematical Statistics","MCMC"]
description: Estimating reliability of a serially configured system under a Bayesian analysis.
output:
  pdf_document: default
  html_document: default
---

$$f(\pi|x) = \frac{f(x|\pi)f(\pi)}{f(x)} \propto f(x|\pi)f(\pi)$$
$$X \sim Bin(n,\pi) \rightarrow f(x|\pi) \sim Bin(x;n,\pi)$$
$$\pi \sim Beta(a,b) \rightarrow f(\pi) = Beta(\pi;a,b)$$
$$f(\pi|x) \propto f(x|\pi)f(\pi) \rightarrow f(\pi|x) \propto Bin(x;n,\pi)\cdot Beta(\pi;a,b)$$
$$\rightarrow f(\pi|x) \propto {n \choose x} \frac{1}{B(a,b)}n^{x+a-1}(1-\pi)^{n-x+b-1}$$
For a series system - 

$$\pi_s \sim \prod_{c=1}^k \pi_c; \quad \pi_c \sim Beta(a_c,b_c)$$ where $s$ and $c$ denote system and component, respectively.

$$\hat{\pi_c} = \frac{n_c - x_c}{n_c}$$
Biasedness of this estimator - 

$$E[\hat{\pi_c}] = \frac{n_c - x_c}{n_c} = \frac{E[n_c] - E[x_c]}{n_c} = \frac{n_c}{n_c} - \frac{n_c - x}{(n_c + 1)n_c} = \frac{n^2_c(n_c + 1) - n_c(n_c - x)}{n^2_c(n_c + 1)}$$
$$= \frac{n^3_c + n^2_c - n^2_c + n_cx_c}{n^2_c(n_c + 1)} = \frac{n^3_c + n_cx_c}{n^2_c(n_c + 1)} = \frac{n_c(n^2_c + x_c)}{n_c(n^2_c + n_c)} = \frac{n^2_c + x_c}{n^2_c + n_c}$$

When $x = 0$ or zero failures occur - 

$$\pi_c \sim Beta(\pi,1)$$
$$a = n; \quad b = 1$$
$$\mu = \frac{a}{a + b} = \frac{n}{n+1}; \quad \sigma^2 = \frac{ab}{(a+b)^2(a+b+1)} = \frac{n}{(n+1)^2(n+2)}$$
Note:

$$Beta(n,1) \rightarrow f(\pi) = \frac{\Gamma(a+b)}{\Gamma(a)\Gamma(b)}\pi^{a-1}(1-\pi)^{b-1} \rightarrow f(\pi) = \frac{\Gamma(n+1)}{\Gamma(n)\Gamma(1)}\pi^{n-1}(1-\pi)^0 = n\pi^{n-1}$$

When $x > 0$ or at least one failure occurs - 

$$\pi_c \sim Beta(n_c,1)$$
$$a = n; \quad b = 1$$






